experiment/Experiment.Steel.Repr.LV_to_M.fst
@@ -1,0 +1,16 @@
+module Experiment.Steel.Repr.LV_to_M
+
+open FStar.Tactics
+
+let bind_g_csm'_res_env_f
+      (env : vprop_list) (b : Type)
+      (f_csm : csm_t env) (f_prd : vprop_list)
+      (g_csm : csm_t (filter_mask (mask_not f_csm) env)) (g_prd : prd_t b)
+  : Lemma (res_env_f (res_env env f_csm f_prd) (bind_g_csm' env f_csm f_prd g_csm) g_prd
+        == res_env_f env (bind_csm env f_csm g_csm) g_prd)
+  =
+    U.funext_eta
+        (res_env_f (res_env env f_csm f_prd) (bind_g_csm' env f_csm f_prd g_csm) g_prd)
+        (res_env_f env (bind_csm env f_csm g_csm) g_prd)
+        (_ by (trefl ())) (_ by (trefl ()))
+        (fun (x : b) -> filter_bind_g_csm' env f_csm f_prd g_csm)
