experiment/Experiment.Steel.Repr.LV_to_M.fsti
@@ -1,0 +1,140 @@
+module Experiment.Steel.Repr.LV_to_M
+
+module U    = Learn.Util
+module L    = FStar.List.Pure
+module M    = Experiment.Steel.Repr.M
+module Veq  = Experiment.Steel.VEquiv
+module Perm = Learn.Permutation
+
+open Learn.List.Mask
+open Experiment.Steel.VPropList
+open Experiment.Steel.Repr.LV
+
+
+let res_env_f (env : vprop_list) (#a : Type) (csm : csm_t env) (prd : prd_t a) (x : a)
+  : vprop_list
+  = res_env env csm (prd x)
+
+let typ_to_M
+      (env : vprop_list)
+      (#a : Type u#a) (t : M.prog_tree a)
+      (csm : csm_t env) (prd : prd_t a)
+  : Type
+  = M.tree_cond t env (res_env_f env csm prd)
+
+let lc_to_M
+      (#env : vprop_list) (#a : Type u#a) (#t : M.prog_tree a)
+      (#csm : csm_t env) (#prd : prd_t a)
+      (lc : lin_cond env t csm prd)
+  : Type
+  = typ_to_M env t csm prd
+
+
+let eij_framed_equiv
+      (env : vprop_list) (pre : M.pre_t) (csm_f : eq_injection_l pre env)
+  : vequiv_perm env L.(pre @ filter_mask (mask_not (eij_trg_mask csm_f)) env)
+  =
+    let m = eij_trg_mask csm_f in
+    filter_mask_perm_append m env;
+    Perm.(pequiv_trans
+      (mask_perm_append m <: vequiv_perm env L.(filter_mask m env @ filter_mask (mask_not m) env))
+      (pequiv_append (eij_equiv csm_f) (pequiv_refl (filter_mask (mask_not m) env))))
+
+let repr_M_of_LV__tcs
+      (env : vprop_list)
+      (a : Type u#a) (pre : M.pre_t) (post : M.post_t a)
+      (csm_f : eq_injection_l pre env)
+  : M.tree_cond_Spec a pre post
+  = {
+    tcs_pre     = env;
+    tcs_post    = res_env_f env (eij_trg_mask csm_f) post;
+    tcs_frame   = filter_mask (mask_not (eij_trg_mask csm_f)) env;
+    tcs_pre_eq  = Veq.vequiv_of_perm (eij_framed_equiv env pre csm_f);
+    tcs_post_eq = (fun x -> Veq.vequiv_refl L.(post x @ filter_mask (mask_not (eij_trg_mask csm_f)) env))
+  }
+
+#push-options "--ifuel 0 --fuel 0"
+let sub_prd_framed_equiv
+      (env  : vprop_list)
+      (csm0 : csm_t env) (prd0 : vprop_list)
+      (csm1 : csm_t (filter_mask (mask_not csm0) env)) (prd1 : vprop_list)
+      (veq  : vequiv_perm (sub_prd env csm0 prd0 csm1) prd1)
+  : vequiv_perm L.(prd0 @ filter_mask (mask_not csm0) env)
+                (res_env env (bind_csm env csm0 csm1) prd1)
+  =
+    let env1 = filter_mask (mask_not csm0) env  in
+    let flt1 = filter_mask csm1 env1            in
+    let flt2 = filter_mask (mask_not csm1) env1 in
+    assert (sub_prd env csm0 prd0 csm1 == L.(prd0 @ flt1));
+    calc (==) {
+      res_env env (bind_csm env csm0 csm1) prd1;
+    == { }
+      L.(prd1 @ filter_mask (mask_not (bind_csm env csm0 csm1)) env);
+    == { filter_bind_csm env csm0 csm1 }
+      L.(prd1 @ flt2);
+    };
+    let f0  : vequiv_perm L.(prd0 @ flt1) prd1 = U.cast _ veq in
+    L.append_assoc prd0 flt1 flt2;
+    let f0' : vequiv_perm L.(prd0 @ flt1 @ flt2) L.(prd1 @ flt2)
+      = U.cast _ (Perm.pequiv_append f0 (Perm.pequiv_refl flt2))
+    in
+    filter_mask_perm_append csm1 env1;
+    let f1  : vequiv_perm env1 L.(flt1 @ flt2)
+       = Perm.perm_cast _ (mask_perm_append csm1)             in
+    let f1' : vequiv_perm L.(prd0 @ env1) L.(prd0 @ flt1 @ flt2)
+      = Perm.pequiv_append (Perm.pequiv_refl prd0) f1
+    in
+    Perm.pequiv_trans f1' f0'
+#pop-options
+
+let repr_M_of_LV__tcs_sub
+      (env : vprop_list)
+      (a : Type u#a) (pre : M.pre_t) (post : M.post_t a)
+      (csm_f : eq_injection_l pre env)
+      (csm1 : csm_t (filter_mask (mask_not (eij_trg_mask csm_f)) env)) (prd1 : prd_t a)
+      (prd_f1 : (x : a) -> Perm.pequiv_list (sub_prd env (eij_trg_mask csm_f) (post x) csm1) (prd1 x))
+  : M.tree_cond_Spec a pre post
+  = {
+    tcs_pre     = env;
+    tcs_post    = res_env_f env (bind_csm env (eij_trg_mask csm_f) csm1) prd1;
+    tcs_frame   = filter_mask (mask_not (eij_trg_mask csm_f)) env;
+    tcs_pre_eq  = Veq.vequiv_of_perm (eij_framed_equiv env pre csm_f);
+    tcs_post_eq = (fun x -> Veq.vequiv_of_perm (
+                           sub_prd_framed_equiv env (eij_trg_mask csm_f) (post x)
+                               csm1 (prd1 x) (Perm.perm_f_of_list (prd_f1 x))))
+  }
+
+val bind_g_csm'_res_env_f
+      (env : vprop_list) (b : Type)
+      (f_csm : csm_t env) (f_prd : vprop_list)
+      (g_csm : csm_t (filter_mask (mask_not f_csm) env)) (g_prd : prd_t b)
+  : Lemma (res_env_f (res_env env f_csm f_prd) (bind_g_csm' env f_csm f_prd g_csm) g_prd
+        == res_env_f env (bind_csm env f_csm g_csm) g_prd)
+
+
+#push-options "--ifuel 1 --fuel 2"
+let rec repr_M_of_LV
+      (#env : vprop_list) (#a : Type u#a) (#t : M.prog_tree a)
+      (#csm : csm_t env) (#prd : prd_t a)
+      (lc : lin_cond env t csm prd)
+  : Pure (lc_to_M lc) (requires lcsub_at_leaves lc) (ensures fun _ -> True) (decreases lc)
+  = match lc with
+  | LCspec env #a #pre #post #req #ens csm_f ->
+      M.TCspec #a #pre #post #req #ens (repr_M_of_LV__tcs env a pre post csm_f)
+  | LCret env #a #x #sl_hint prd csm_f ->
+      M.TCret #a #x #sl_hint
+          env (fun x' -> L.(prd x' @ filter_mask (mask_not (eij_trg_mask csm_f)) env))
+          (Veq.vequiv_of_perm (eij_framed_equiv env (prd x) csm_f))
+  | LCbind env #a #b #f #g f_csm f_prd cf g_csm g_prd cg ->
+      M.TCbind #a #b #f #g env (res_env_f env f_csm f_prd) (res_env_f env (bind_csm env f_csm g_csm) g_prd)
+          (repr_M_of_LV cf)
+          (fun (x : a) ->
+            (**) bind_g_csm'_res_env_f env b f_csm (f_prd x) g_csm g_prd;
+            repr_M_of_LV (cg x))
+  | LCsub env #a0 #f0 csm0 prd0 cf csm1 prd1 prd_f1 ->
+      let LCspec env #a #pre #post #req #ens csm_f = cf in
+      let prd_f1 (x : a) : Perm.pequiv_list (sub_prd env (eij_trg_mask csm_f) (post x) csm1) (prd1 x)
+            = U.cast _ (prd_f1 x)
+      in
+      M.TCspec #a #pre #post #req #ens (repr_M_of_LV__tcs_sub env a pre post csm_f csm1 prd1 prd_f1)
+#pop-options
